{
 "cells": [
  {
   "cell_type": "markdown",
   "metadata": {},
   "source": [
    "Stochastic Volatilty Models\n",
    "\n",
    "#### Home work 2\n",
    "\n",
    "---"
   ]
  },
  {
   "cell_type": "markdown",
   "metadata": {},
   "source": [
    "The file must be sent to **stoch-vol-23-fall@yandex.ru** with topic \"stoch-vol HW2\". WARNING: topic is important! Inbox will be filtered automatcally based on exact match. Please zip all files into one folder and rename it as \"SurnameName_HW2\" before sending.\n",
    "\n",
    "Deadline: 25th of December, 23:59.\n",
    "\n",
    "If you have any questions feel free to ask in Telegram https://t.me/v_antipov or https://t.me/igortao.\n",
    "\n",
    "Full name: Cherepakhin Ivan\n",
    "\n",
    "Faculty: MechMat MSU"
   ]
  },
  {
   "cell_type": "markdown",
   "metadata": {},
   "source": [
    "---"
   ]
  },
  {
   "cell_type": "markdown",
   "metadata": {},
   "source": [
    "### Problem 1 (40 points)"
   ]
  },
  {
   "cell_type": "markdown",
   "metadata": {},
   "source": [
    "Let $S^{(r)}$ be the underlying process from the CEV model with interest rate $r$, that is satisfying the SDE\n",
    "\n",
    "$$dS^{(r)}_t = r S^{(r)}_t dt + \\sigma (S^{(r)}_t)^{\\beta} dW_t, \\quad S^{(r)}_0 = s > 0.$$\n",
    "\n",
    "Show that under the time-change \n",
    "$$\\tau(t) = \\frac{e^{2r(\\beta - 1)t} - 1}{2r(\\beta - 1)},$$\n",
    "\n",
    "the following relationship holds \n",
    "\n",
    "$$S^{(r)}_t \\stackrel{d}{=} e^{rt} S^{(0)}_{\\tau(t)}.$$"
   ]
  },
  {
   "cell_type": "markdown",
   "metadata": {},
   "source": [
    "*Instructions:*"
   ]
  },
  {
   "cell_type": "markdown",
   "metadata": {},
   "source": [
    "**1**. üß† <span style=\"color:blue\">(10 points)</span>  Show that the discounted underlying process process $X_t := e^{-rt} S_t^{(r)}$ satisfies the SDE\n",
    "\n",
    "$$dX_t = \\sigma e^{r(\\beta - 1)t} X_t^{\\beta} dW_t.$$"
   ]
  },
  {
   "cell_type": "markdown",
   "metadata": {},
   "source": [
    "YOUR ANSWER HERE"
   ]
  },
  {
   "cell_type": "markdown",
   "metadata": {},
   "source": [
    "–°–¥–µ–ª–∞–µ–º –∑–∞–º–µ–Ω—É –≤—Ä–µ–º–µ–Ω–∏ –∏–∑ –≤—ã—à–µ."
   ]
  },
  {
   "cell_type": "markdown",
   "metadata": {},
   "source": [
    "\n",
    "$$X_t = f (t, S_t), f(t, s) = e^{-rt}s, f_t = -re^{-rt}s = -rf, f_s = f/s, f_{ss} = 0 $$\n",
    "\n",
    "$$ df(t, S^{(r)}_t) = f_tdt + f_sdS^{(r)}_t + 0.5f_{ss} dS^{(r)}_t dS^{(r)}_t = $$\n",
    "$$ = -rfdt + \\frac{1}{s}f(rS^{(r)}_tdt + \\sigma (S^{(r)}_t)^{\\beta} dW_t) = $$\n",
    "$$ = -re^{-rt}S^{(r)}_tdt + e^{-rt}(rS^{(r)}_tdt + \\sigma (S^{(r)}_t)^{\\beta} dW_t) = $$\n",
    "$$ = e^{-rt} \\sigma (S^{(r)}_t)^{\\beta} dW_t = $$\n",
    "$$ = e^{-rt} \\sigma e^{rt \\beta }  e^{-rt \\beta }(S^{(r)}_t)^{\\beta} dW_t = $$\n",
    "$$ = \\sigma e^{r( \\beta - 1)t} X^{\\beta}_t dW_t$$"
   ]
  },
  {
   "cell_type": "markdown",
   "metadata": {},
   "source": [
    "**2**. üß† <span style=\"color:blue\">(10 points)</span>  Show that the time-changed zero-rate underlying process process $\\widetilde X_t := S_{\\tau(t)}^{(0)}$ can be represented as\n",
    "\n",
    "$$\\widetilde X_t = s_0 + \\int_{0}^{t} \\sigma (S^{(0)}_{\\tau(u)})^{\\beta}dW_{\\tau(u)}.$$\n",
    "\n",
    "\n",
    "Then show that $W_{\\tau(u)}$ can be represented as \n",
    "$$W_{\\tau(u)} = \\int_{0}^{u} \\sqrt{\\tau'(v)} d \\widetilde W_v,$$\n",
    "\n",
    "where $\\tilde W_v$ is some Brownian motion. "
   ]
  },
  {
   "cell_type": "markdown",
   "metadata": {},
   "source": [
    "YOUR ANSWER HERE"
   ]
  },
  {
   "cell_type": "markdown",
   "metadata": {},
   "source": [
    "–°–¥–µ–ª–∞–µ–º –∑–∞–º–µ–Ω—É –≤—Ä–µ–º–µ–Ω–∏ –≤ –∏–Ω—Ç–µ–≥—Ä–∞–ª–µ"
   ]
  },
  {
   "cell_type": "markdown",
   "metadata": {},
   "source": [
    "$$ dS^{(0)}_t = \\sigma (S^{(0)}_t)^{\\beta} dW_t, dS^{(0)}_{\\tau(t)} = \\sigma (S^{(0)}_{\\tau(t)})^{\\beta} dW_t$$\n",
    "$$ S^{(0)}_{\\tau(t)} = s_0 + \\int_{\\tau(0)}^{\\tau(t)} \\sigma (S^{(0)}_{\\tau})^{\\beta}dW_{\\tau} $$"
   ]
  },
  {
   "cell_type": "markdown",
   "metadata": {},
   "source": [
    "$$ S^{(0)}_{\\tau(t)} = s_0 + \\int_{0}^{t} \\sigma (S^{(0)}_t)^{\\beta} \\sqrt{\\tau'(t)} dW_t\n",
    "= s_0 + \\int_{0}^{t} \\sigma (S^{(0)}_t)^{\\beta} dW_{\\tau(t)} = \\widetilde X_t$$"
   ]
  },
  {
   "cell_type": "markdown",
   "metadata": {},
   "source": [
    "**3**. üß† <span style=\"color:blue\">(10 points)</span>  Show that $\\widetilde X_t$ satisfies the SDE \n",
    "\n",
    "$$d \\widetilde X_t = \\sigma e^{r (\\beta - 1) t } \\widetilde X_t^{\\beta} d \\widetilde W_t.$$"
   ]
  },
  {
   "cell_type": "markdown",
   "metadata": {},
   "source": [
    "YOUR ANSWER HERE"
   ]
  },
  {
   "cell_type": "markdown",
   "metadata": {},
   "source": [
    "–ò–∑ –ø—Ä–µ–¥—ã–¥—É—â–µ–≥–æ"
   ]
  },
  {
   "cell_type": "markdown",
   "metadata": {},
   "source": [
    "$$ \\widetilde X_t = s_0 + \\int_{0}^{t} \\sigma (S^{(0)}_t)^{\\beta} \\sqrt{\\tau'(t)} dW_t $$\n",
    "$$d\\widetilde X_t = \\sigma (S^{(0)}_t)^{\\beta} \\sqrt{\\tau'(t)} dW_t $$\n",
    "$$ (\\widetilde X_t)^{\\beta} = (S^{(0)}_t)^{\\beta} $$\n",
    "$$ \\sqrt{\\tau'(t)} = e^{r(\\beta - 1)t} $$"
   ]
  },
  {
   "cell_type": "markdown",
   "metadata": {},
   "source": [
    "–°–æ–æ—Ç–≤–µ—Ç—Å–≤—Ç–µ–Ω–Ω–æ –ø–æ–ª—É—á–∞–µ–º"
   ]
  },
  {
   "cell_type": "markdown",
   "metadata": {},
   "source": [
    "$$ d \\widetilde X_t = \\sigma e^{r (\\beta - 1) t } \\widetilde X_t^{\\beta} d \\widetilde W_t  $$"
   ]
  },
  {
   "cell_type": "markdown",
   "metadata": {},
   "source": [
    "**4**. üß† <span style=\"color:blue\">(10 points)</span>  Conclude that \n",
    "\n",
    "$$X_t \\stackrel{d}{=} \\widetilde X_t.$$"
   ]
  },
  {
   "cell_type": "markdown",
   "metadata": {},
   "source": [
    "YOUR ANSWER HERE"
   ]
  },
  {
   "cell_type": "markdown",
   "metadata": {},
   "source": [
    "–•–æ—Ç–∏–º –∏—Å–ø–æ–ª—å–∑–æ–≤–∞—Ç—å —Ç–µ–æ—Ä–µ–º—É –ò—Ç–æ –æ —Å–∏–ª—å–Ω–æ–º –µ–¥–∏–Ω—Å—Ç–≤–µ–Ω–Ω–æ–º —Ä–µ—à–µ–Ω–∏–∏. –î–ª—è —ç—Ç–æ–≥–æ –Ω—É–∂–Ω–æ –ø–æ–¥–æ–±—Ä–∞—Ç—å —É–¥–æ–±–Ω—ã–µ –ø–∞—Ä–∞–º–µ—Ç—Ä—ã."
   ]
  },
  {
   "cell_type": "markdown",
   "metadata": {},
   "source": [
    "–ó–Ω–∞–µ–º, —á—Ç–æ $ d \\widetilde X_t = \\sigma e^{r (\\beta - 1) t } \\widetilde X_t^{\\beta} d \\widetilde W_t$ –∏ $ d  X_t = \\sigma e^{r (\\beta - 1) t }  X_t^{\\beta} d W_t $."
   ]
  },
  {
   "cell_type": "markdown",
   "metadata": {},
   "source": [
    "---"
   ]
  },
  {
   "cell_type": "markdown",
   "metadata": {},
   "source": [
    "### Problem 2 (20 points)"
   ]
  },
  {
   "cell_type": "markdown",
   "metadata": {},
   "source": [
    "Let $S$ be the underlying process from the CEV model with zero interest rate, that is satisfying the SDE\n",
    "\n",
    "$$dS_t = \\sigma (S_t)^{\\beta} dW_t, \\quad S_0 = s > 0.$$\n",
    "\n",
    "Show that the process $$X_t := \\frac{S^{2(1 - \\beta)}_t}{\\sigma^2 (1 - \\beta)^2}$$\n",
    "\n",
    "is a square of the Bessel proceess of dimension $\\delta = (1 - 2 \\beta) / (1 - \\beta)$, i.e. satisfies the SDE \n",
    "\n",
    "$$dX_t = \\delta dt + 2 \\sqrt{|X_t|} dW_t.$$"
   ]
  },
  {
   "cell_type": "markdown",
   "metadata": {},
   "source": [
    "YOUR ANSWER HERE"
   ]
  },
  {
   "cell_type": "markdown",
   "metadata": {},
   "source": [
    "$$ X_t = f(t, S_t), f = \\frac{s^{2(1 - \\beta)}}{\\sigma^2 (1 - \\beta)^2}, f_t = 0, f_s = 2(1 - \\beta) \\frac{s^{2(1 - \\beta) - 1}}{\\sigma^2 (1 - \\beta)^2}, f_{ss} = \\frac{2(2(1 - \\beta) - 1) s^{-2\\beta}}{\\sigma^2 (1 - \\beta)}$$\n",
    "$$ dX_t = f_s dS_t + 0.5f_{ss} dS_t dS_t = \\frac{2 S^{2(1 - \\beta) - 1}_t}{\\sigma^2 (1 - \\beta)} \\sigma S^{\\beta}_t dW_t + \\frac{2(2(1 - \\beta) - 1)}{2 \\sigma^2 (1 - \\beta)} S^{-2\\beta}_t \\sigma^2 S^{2\\beta}_t dt = $$\n",
    "$$ = \\frac{1 - 2\\beta}{1 - \\beta} dt + \\frac{2}{\\sigma (1 - \\beta)}S^{1 - \\beta}_t dW_t = \\delta dt + 2 \\sqrt{\\frac{S^{2(1 - \\beta)}_t}{\\sigma^2 (1 - \\beta)^2}}dW_t = \\delta dt + 2 \\sqrt{|X_t|} dW_t$$"
   ]
  },
  {
   "cell_type": "markdown",
   "metadata": {},
   "source": [
    "---"
   ]
  },
  {
   "cell_type": "markdown",
   "metadata": {},
   "source": [
    "### Problem 3 (40 points)"
   ]
  },
  {
   "cell_type": "markdown",
   "metadata": {},
   "source": [
    "In Heston model under the martingale measure (the measure under which all underlying assets are martinagales w.r.t the money-market account $dB_t = B_t r dt$, $B_0 = 1$) the price process is given by a system of SDE \n",
    "\n",
    "$$dS_t = S_t (r dt + \\sqrt{V_t} d W^{S}_t), \\quad S_0 = s > 0,$$\n",
    "$$d V_t = \\kappa (\\bar V - V_t) dt + \\gamma \\sqrt{V_t} \\left[ \\rho d W^{S}_t + \\sqrt{1 - \\rho^2} d W^{V}_t \\right], \\quad V_0 = v > 0.$$\n",
    "\n",
    "Derive the model dynamics under the the stock-measure $\\mathbb{Q}^{S}$, under which all assets are martingales w.r.t. the stock price $S_t$. "
   ]
  },
  {
   "cell_type": "markdown",
   "metadata": {},
   "source": [
    "*Instructions:*"
   ]
  },
  {
   "cell_type": "markdown",
   "metadata": {},
   "source": [
    "**1**. üß† <span style=\"color:blue\">(10 points)</span> Define a process $Y_t := B_t/S_t$ and show that its dynamics are given by\n",
    "\n",
    "$$dY_t = Y_t (V_t dt - \\sqrt{V_t} dW^{S}_t), \\quad Y_0 = 1/S_0.$$"
   ]
  },
  {
   "cell_type": "markdown",
   "metadata": {},
   "source": [
    "YOUR ANSWER HERE"
   ]
  },
  {
   "cell_type": "markdown",
   "metadata": {},
   "source": [
    "$$ Y_t = f(t, B_t, S_t), f(t, b, s) = \\frac{b}{s}, f_t = 0, f_s = - \\frac{b}{s^2}, f_b = \\frac{1}{s}, f_{ss} = \\frac{2b}{s^3}, f_{bb} = 0, f_{bs} = f_{sb} = \\frac{2}{s^3}$$\n",
    "$$ dY_t = df(t, B_t, S_t) = - \\frac{B_t}{S^{2}_t} dS_t + \\frac{1}{S_t} dB_t + \\frac{1}{2} \\frac{2B_t}{S^{3}_t} (dS_t)^2 + \\frac{2}{S^{3}_t} dS_tdB_t = $$\n",
    "$$ = - \\frac{B_t}{S^{2}_t} S_t(rdt + \\sqrt{V_t} dW^{s}_t) + \\frac{1}{S_t} B_trdt + \\frac{1}{2} \\frac{2B_t}{S^{3}_t} S^{2}_t V_t dt + \\frac{2}{S^{3}_t} 0 = $$\n",
    "$$ = - \\frac{B_t}{S_t} rdt - \\frac{B_t}{S_t} \\sqrt{V_t} dW^{s}_t + \\frac{B_t}{S_t} rdt + \\frac{B_t}{S_t} V_t dt = \\frac{1}{S_t} dt B_tV_t - \\frac{B_t}{S_t} \\sqrt{V_t} dW^{s}_t = $$\n",
    "$$ = \\frac{B_t}{S_t} (V_tdt - \\sqrt{V_t} dW^{s}_t) = Y_t ( V_tdt - \\sqrt{V_t} dW^{s}_t ) $$\n",
    "$$ Y_0 = \\frac{B_0}{S_0} = \\frac{1}{S_0}$$"
   ]
  },
  {
   "cell_type": "markdown",
   "metadata": {},
   "source": [
    "**2**. üß† <span style=\"color:blue\">(10 points)</span> Define another Brownian motion, $\\tilde W^{S}_t$, for which process $Y_t$ becomes a martingale. "
   ]
  },
  {
   "cell_type": "markdown",
   "metadata": {},
   "source": [
    "YOUR ANSWER HERE"
   ]
  },
  {
   "cell_type": "markdown",
   "metadata": {},
   "source": [
    "–û–ø—Ä–µ–¥–µ–ª–∏–º –±—Ä –¥–≤–∏–∂ –∏–∑ —Ç–µ–æ—Ä–µ–º—ã –≥–∏—Ä—Å–∞–Ω–æ–≤–∞ –∏ –ª–µ–≤–∏ —Ö–∞—Ä–∞–∫—Ç–µ—Ä, –≥–¥–µ $(\\int_{0}^{t} (\\sqrt{V_t})^2 dt < \\infty)$."
   ]
  },
  {
   "cell_type": "markdown",
   "metadata": {},
   "source": [
    "$$ dY_t = Y_t V_t dt - Y_t \\sqrt{V_t} dW^{s}_t = Y_t \\sqrt{V_t} ( \\sqrt{V_t} dt - dW^{s}_t) = \\alpha_t d \\widetilde W^{s}_t $$\n",
    "$$ \\alpha_t =  Y_t \\sqrt{V_t} , d \\widetilde W^{s}_t = \\sqrt{V_t} dt - dW^{s}_t$$"
   ]
  },
  {
   "cell_type": "markdown",
   "metadata": {},
   "source": [
    "**3**. üß† <span style=\"color:blue\">(10 points)</span> Use the derived measure transformation to show that the Heston model under the $\\mathbb{Q}^S$ measure reads\n",
    "\n",
    "$$dS_t = S_t ((r + V_t)dt - \\sqrt{V_t} d \\widetilde W^{S}_t), \\quad S_0 = s > 0,$$\n",
    "$$d V_t = \\kappa^{*} (\\bar V^{*} - V_t) dt + \\gamma \\sqrt{V_t} \\left[ - \\rho d \\widetilde W^{S}_t + \\sqrt{1 - \\rho^2} d W^{V}_t \\right], \\quad V_0 = v > 0,$$\n",
    "\n",
    "where $\\kappa^{*} = \\kappa - \\rho \\gamma$, $\\bar V^{*} = \\kappa \\bar V / (\\kappa - \\rho \\gamma)$. "
   ]
  },
  {
   "cell_type": "markdown",
   "metadata": {},
   "source": [
    "YOUR ANSWER HERE"
   ]
  },
  {
   "cell_type": "markdown",
   "metadata": {},
   "source": [
    "$$ S_t ((r + V_t)dt - \\sqrt{V_t} d \\widetilde W^{S}_t) = S_t ((r + V_t) dt - V_t dt + \\sqrt{V_t} dW^{s}_t ) = S_t ( rdt + \\sqrt{V_t} dW^{s}_t) = dS_t $$\n",
    "\n",
    "$$ \\kappa^{*} (\\bar V^{*} - V_t) dt + \\gamma \\sqrt{V_t} \\left[ - \\rho d \\widetilde W^{S}_t + \\sqrt{1 - \\rho^2} d W^{V}_t \\right] = $$ \n",
    "$$ = (\\kappa - \\rho \\gamma) (\\frac{\\kappa \\bar V}{(\\kappa - \\rho \\gamma)} - V_t)dt + \\gamma \\sqrt{V_t} (-\\rho \\sqrt{V_t} dt + \\rho dW^{s}_t + \\sqrt{1 - \\rho^2} dW^{V}_t) = $$ \n",
    "$$ = \\kappa \\bar V dt - (\\kappa - \\rho \\gamma) V_t dt - \\rho \\gamma V_t dt + \\gamma \\sqrt{V_t} ( \\rho dW^{s}_t + \\sqrt{1 - \\rho^2} dW^{V}_t) = $$ \n",
    "$$ = \\kappa \\bar V dt - \\kappa V_t dt + \\gamma \\sqrt{V_t} (\\rho dW^{s}_t + \\sqrt{1 - \\rho^2}dW^{V}_t) $$\n",
    "$$= \\kappa dt(\\bar V - V_t) + \\gamma \\sqrt{V_t} (\\rho dW^{s}_t + \\sqrt{1 - \\rho^2} dW^{V}_t) = dV_t $$"
   ]
  },
  {
   "cell_type": "markdown",
   "metadata": {},
   "source": [
    "**4**. üß† <span style=\"color:blue\">(10 points)</span> Use the transform $d \\widehat  W^{S}_t = - d \\widetilde W^{S}_t$ to obtain the final equations. "
   ]
  },
  {
   "cell_type": "markdown",
   "metadata": {},
   "source": [
    "YOUR ANSWER HERE"
   ]
  },
  {
   "cell_type": "markdown",
   "metadata": {},
   "source": [
    "–ü—Ä–æ–¥–∞–ª–∂–∞—è –ø—Ä–µ–¥—ã–¥—É—â–µ–µ,\n",
    "$$ dS_t = S_t((r + V_t)dt + \\sqrt{V_t} d \\widehat W^{s}_t $$\n",
    "$$ dV_t = \\kappa^{*} (\\bar V^{*} - V_t) dt + \\gamma \\sqrt{V_t} \\left[ \\rho d \\widehat W^{S}_t + \\sqrt{1 - \\rho^2} d W^{V}_t \\right] $$\n"
   ]
  },
  {
   "cell_type": "markdown",
   "metadata": {},
   "source": []
  }
 ],
 "metadata": {
  "kernelspec": {
   "display_name": "Python 3",
   "language": "python",
   "name": "python3"
  },
  "language_info": {
   "codemirror_mode": {
    "name": "ipython",
    "version": 3
   },
   "file_extension": ".py",
   "mimetype": "text/x-python",
   "name": "python",
   "nbconvert_exporter": "python",
   "pygments_lexer": "ipython3",
   "version": "3.8.5"
  },
  "orig_nbformat": 4
 },
 "nbformat": 4,
 "nbformat_minor": 2
}
